dafny_code/bool.dfy
@@ -1,37 +1,37 @@
-datatype Qubit = Qubit(index: nat)
+datatype Nor = Nor(k: bv1)
+datatype Had = Had(0: bv1, 1: bv1)
 datatype En2 = En2(k: nat, j: nat)
 datatype En1 = En1(k: nat)
 
-function method pow2(N:nat):int
+function pow2(N:nat):int
   ensures pow2(N) > 0
 {
 	if (N==0) then 1 else 2 * pow2(N-1)
 }
 
-function method {:axiom} sqrt(a:real) :real 
+function {:axiom} sqrt(a:real) :real 
     requires a > 0.0
     ensures sqrt(a) > 0.0
 
-function method {:axiom} a(j: nat): real
-function method {:axiom} ph(j: nat): real
-function method {:axiom} omega(a:real, n:nat): real
-function method {:axiom} cos(a:real): real
+function {:axiom} a(j: nat): real
+function {:axiom} ph(j: nat): real
+function {:axiom} omega(a:real, n:nat): real
+function {:axiom} cos(a:real): real
 
-//WLOG we assume theta is in [0,pi/2]
-function method {:axiom} sin(a:real): real
+//WLOG we assume theta is in [0,pi/2)
+function {:axiom} sin(a:real): real
     ensures sin(a) != 0.0
 
-// function method phi(n: nat): (En1 -> real)
+// function phi(n: nat): (En1 -> real)
 //     requires n >= 0
 //     ensures forall state :: phi(n)(state) == 
 //              if 0 <= state.k < pow2(n)
 //              then (1.0/sqrt(pow2(n) as real)) * a(state.k) 
 //              else 0.0
 //assuming that a(k) is the amplitude of the k-th state after applying unitary operation A
-function method alpha(n: nat, f: nat -> bv1): (En1 -> real)
+function alpha(n: nat, f: nat -> bv1): (En1 -> real)
     requires n >= 0
-    ensures forall state :: alpha(n, f)(state) == 
-      if state.k < pow2(n) && f(state.k) == 1 then
+    ensures forall state :: alpha(n, f)(state) == if state.k < pow2(n) && f(state.k) == 1 then
         (1.0/sqrt(pow2(n) as real)) * a(state.k) 
       else if state.k < pow2(n) && f(state.k) == 0 then
         0.0
@@ -47,27 +47,26 @@ function method alpha(n: nat, f: nat -> bv1): (En1 -> real)
             0.0 
         }
 
-function method beta(n: nat, f: nat -> bv1): (En1 -> real)
+function beta(n: nat, f: nat -> bv1): (En1 -> real)
     requires n >= 0
-    ensures forall state :: beta(n, f)(state) == 
-      if state.k < pow2(n) && f(state.k) == 0 then
+    ensures forall state :: beta(n, f)(state) == if state.k < pow2(n) && f(state.k) == 0 then
         (1.0/sqrt(pow2(n) as real)) * a(state.k) 
       else if state.k < pow2(n) && f(state.k) == 0 then
         0.0
       else 
         0.0
+        
 
-function method phi(n: nat, alpha: (En1 -> real), beta: (En1 -> real), theta: real): (En1 -> real)
+function phi(n: nat, alpha: (En1 -> real), beta: (En1 -> real), theta: real): (En1 -> real)
     requires n >= 0
-    ensures forall state :: phi(n, alpha, beta, theta)(state) == 
-             if 0 <= state.k < pow2(n)
-             then sin(theta)*alpha(state) + cos(theta)*beta(state)
+    ensures forall state :: phi(n, alpha, beta, theta)(state) == if 0 <= state.k < pow2(n) then 
+            sin(theta)*alpha(state) + cos(theta)*beta(state)
              else 0.0
 
 
 
 //properties of t unitary operation
-function method VU(alpha: (En1 -> real), beta: (En1 -> real), theta: real, n: nat, t: nat): (En1 -> real)
+function VU(alpha: (En1 -> real), beta: (En1 -> real), theta: real, n: nat, t: nat): (En1 -> real)
     ensures forall state :: VU(alpha, beta, theta, n, t)(state) == 
       if state.k < pow2(n) then
         sin((2*t+1) as real *theta)*alpha(state) + cos((2*t+1) as real * theta)*beta(state)
